SP1Operations/ALUTypeReader.lean
@@ -1,0 +1,87 @@
+import SP1Foundations
+import SP1Operations.MemoryConsistency
+import LeanRV32D.RiscvRegs
+
+open LeanRV32D.Functions
+
+--- A Reader that only accesses values of type `T`.
+structure ALUTypeReader where
+  op_a : BabyBear
+  op_a_memory : MemoryAccessInSharedCols
+  op_a_0 : BabyBear
+  op_b : BabyBear
+  op_b_memory : MemoryAccessInSharedCols
+  op_c : Word BabyBear
+  op_c_memory : MemoryAccessInSharedCols
+  imm_c : BabyBear
+
+namespace ALUTypeReader
+
+def constraints
+  (shard clk pc opcode: BabyBear)
+  (op_a_write_value : Word BabyBear)
+  (cols : ALUTypeReader)
+  (is_real : BabyBear)
+  : List SP1Constraint :=
+    let E0 : BabyBear := is_real - 1
+    let E2 : BabyBear := is_real * E0
+    let E4 : BabyBear := is_real - 1
+    let E6 : BabyBear := cols.imm_c - 0
+    let E8 : BabyBear := E4 * E6
+    let E10 : BabyBear := 0 + cols.op_b
+    let E12 : BabyBear := op_a_write_value[0] - 0
+    let E14 : BabyBear := cols.op_a_0 * E12
+    let E16 : BabyBear := op_a_write_value[1] - 0
+    let E18 : BabyBear := cols.op_a_0 * E16
+    let E20 : BabyBear := clk + 3
+    let E22 : BabyBear := is_real - 1
+    let E24 : BabyBear := is_real * E22
+    let E26 : BabyBear := E20 - cols.op_a_memory.access_timestamp.prev_clk
+    let E28 : BabyBear := E26 - 1
+    let E30 : BabyBear := E28 - cols.op_a_memory.access_timestamp.diff_low_limb
+    let E32 : BabyBear := E30 * 2013143041
+    let E34 : BabyBear := clk + 2
+    let E36 : BabyBear := is_real - 1
+    let E38 : BabyBear := is_real * E36
+    let E40 : BabyBear := E34 - cols.op_b_memory.access_timestamp.prev_clk
+    let E42 : BabyBear := E40 - 1
+    let E44 : BabyBear := E42 - cols.op_b_memory.access_timestamp.diff_low_limb
+    let E46 : BabyBear := E44 * 2013143041
+    let E48 : BabyBear := clk + 1
+    let E50 : BabyBear := is_real - cols.imm_c
+    let E52 : BabyBear := E50 - 1
+    let E54 : BabyBear := E50 * E52
+    let E56 : BabyBear := E48 - cols.op_c_memory.access_timestamp.prev_clk
+    let E58 : BabyBear := E56 - 1
+    let E60 : BabyBear := E58 - cols.op_c_memory.access_timestamp.diff_low_limb
+    let E62 : BabyBear := E60 * 2013143041
+    let E64 : BabyBear := cols.op_c_memory.prev_value[0] - cols.op_c[0]
+    let E66 : BabyBear := cols.imm_c * E64
+    let E68 : BabyBear := cols.op_c_memory.prev_value[1] - cols.op_c[1]
+    let E70 : BabyBear := cols.imm_c * E68
+
+    [
+      .assertZero E2,
+      .assertZero E8,
+      .assertZero E14,
+      .assertZero E18,
+      .assertZero E24,
+      .send (.byte (ByteOpcode.ofNat 6) cols.op_a_memory.access_timestamp.diff_low_limb 14 0) is_real,
+      .send (.byte (ByteOpcode.ofNat 6) E32 14 0) is_real,
+      .send (.memory shard cols.op_a_memory.access_timestamp.prev_clk cols.op_a cols.op_a_memory.prev_value[0] cols.op_a_memory.prev_value[1]) is_real,
+      .receive (.memory shard E20 cols.op_a op_a_write_value[0] op_a_write_value[1]) is_real,
+      .assertZero E38,
+      .send (.byte (ByteOpcode.ofNat 6) cols.op_b_memory.access_timestamp.diff_low_limb 14 0) is_real,
+      .send (.byte (ByteOpcode.ofNat 6) E46 14 0) is_real,
+      .send (.memory shard cols.op_b_memory.access_timestamp.prev_clk cols.op_b cols.op_b_memory.prev_value[0] cols.op_b_memory.prev_value[1]) is_real,
+      .receive (.memory shard E34 cols.op_b cols.op_b_memory.prev_value[0] cols.op_b_memory.prev_value[1]) is_real,
+      .assertZero E54,
+      .send (.byte (ByteOpcode.ofNat 6) cols.op_c_memory.access_timestamp.diff_low_limb 14 0) E50,
+      .send (.byte (ByteOpcode.ofNat 6) E62 14 0) E50,
+      .send (.memory shard cols.op_c_memory.access_timestamp.prev_clk cols.op_c[0] cols.op_c_memory.prev_value[0] cols.op_c_memory.prev_value[1]) E50,
+      .receive (.memory shard E48 cols.op_c[0] cols.op_c_memory.prev_value[0] cols.op_c_memory.prev_value[1]) E50,
+      .assertZero E66,
+      .assertZero E70
+    ]
+
+end ALUTypeReader
